Phi_System/IDE_CP_Applications1.thy
@@ -361,7 +361,7 @@ lemma [\<phi>reason %\<A>_map_each_item]:
   by simp
 
 lemma [\<phi>reason %\<A>_map_each_item]:
-  \<open> (\<c>\<o>\<n>\<d>\<i>\<t>\<i>\<o>\<n> Q \<Longrightarrow> X \<t>\<r>\<a>\<n>\<s>\<f>\<o>\<r>\<m>\<s> Y \<w>\<i>\<t>\<h> P @action \<A>_map_each_item A)
+  \<open> \<c>\<o>\<n>\<d>\<i>\<t>\<i>\<o>\<n> Q \<longrightarrow> (X \<t>\<r>\<a>\<n>\<s>\<f>\<o>\<r>\<m>\<s> Y \<w>\<i>\<t>\<h> P @action \<A>_map_each_item A)
 \<Longrightarrow> X \<s>\<u>\<b>\<j> Q \<t>\<r>\<a>\<n>\<s>\<f>\<o>\<r>\<m>\<s> Y \<s>\<u>\<b>\<j> Q \<w>\<i>\<t>\<h> P @action \<A>_map_each_item A\<close>
   unfolding Action_Tag_def Premise_def Transformation_def
   by simp blast
