Phi_System/Phi_BI.thy
@@ -1785,22 +1785,22 @@ lemma [\<phi>reason %ToA_red]:
   unfolding Transformation_def by simp
 
 lemma [\<phi>reason %ToA_subj+10]: (*THINK: add Q in P, is good or not?*)
-  "(\<p>\<r>\<e>\<m>\<i>\<s>\<e> Q \<Longrightarrow> T \<t>\<r>\<a>\<n>\<s>\<f>\<o>\<r>\<m>\<s> U \<w>\<i>\<t>\<h> P )
+  "\<c>\<o>\<n>\<d>\<i>\<t>\<i>\<o>\<n> Q \<longrightarrow> (T \<t>\<r>\<a>\<n>\<s>\<f>\<o>\<r>\<m>\<s> U \<w>\<i>\<t>\<h> P )
 \<Longrightarrow> T \<s>\<u>\<b>\<j> Q \<t>\<r>\<a>\<n>\<s>\<f>\<o>\<r>\<m>\<s> U \<w>\<i>\<t>\<h> P"
   unfolding Transformation_def Premise_def by simp blast
 
 lemma [\<phi>reason %ToA_subj+20]:
-  "(\<p>\<r>\<e>\<m>\<i>\<s>\<e> Q \<Longrightarrow> T \<t>\<r>\<a>\<n>\<s>\<f>\<o>\<r>\<m>\<s> U \<r>\<e>\<m>\<a>\<i>\<n>\<s>[C] R \<w>\<i>\<t>\<h> P)
+  "\<c>\<o>\<n>\<d>\<i>\<t>\<i>\<o>\<n> Q \<longrightarrow> (T \<t>\<r>\<a>\<n>\<s>\<f>\<o>\<r>\<m>\<s> U \<r>\<e>\<m>\<a>\<i>\<n>\<s>[C] R \<w>\<i>\<t>\<h> P)
 \<Longrightarrow> T \<s>\<u>\<b>\<j> Q \<t>\<r>\<a>\<n>\<s>\<f>\<o>\<r>\<m>\<s> U \<r>\<e>\<m>\<a>\<i>\<n>\<s>[C] R \<s>\<u>\<b>\<j> Q \<w>\<i>\<t>\<h> P"
   unfolding Transformation_def Premise_def by simp blast
 
 lemma [\<phi>reason %ToA_subj+10]:
-  \<open>(\<p>\<r>\<e>\<m>\<i>\<s>\<e> Q \<Longrightarrow> W * T \<t>\<r>\<a>\<n>\<s>\<f>\<o>\<r>\<m>\<s> U \<w>\<i>\<t>\<h> P )
+  \<open>\<c>\<o>\<n>\<d>\<i>\<t>\<i>\<o>\<n> Q \<longrightarrow> (W * T \<t>\<r>\<a>\<n>\<s>\<f>\<o>\<r>\<m>\<s> U \<w>\<i>\<t>\<h> P )
 \<Longrightarrow> W * (T \<s>\<u>\<b>\<j> Q) \<t>\<r>\<a>\<n>\<s>\<f>\<o>\<r>\<m>\<s> U \<w>\<i>\<t>\<h> P \<close>
   unfolding Transformation_def Premise_def by simp blast
 
 lemma [\<phi>reason %ToA_subj+20]:
-  "(\<p>\<r>\<e>\<m>\<i>\<s>\<e> Q \<Longrightarrow> W * T \<t>\<r>\<a>\<n>\<s>\<f>\<o>\<r>\<m>\<s> U \<r>\<e>\<m>\<a>\<i>\<n>\<s>[C] R \<w>\<i>\<t>\<h> P)
+  "\<c>\<o>\<n>\<d>\<i>\<t>\<i>\<o>\<n> Q \<longrightarrow> (W * T \<t>\<r>\<a>\<n>\<s>\<f>\<o>\<r>\<m>\<s> U \<r>\<e>\<m>\<a>\<i>\<n>\<s>[C] R \<w>\<i>\<t>\<h> P)
 \<Longrightarrow> W * (T \<s>\<u>\<b>\<j> Q) \<t>\<r>\<a>\<n>\<s>\<f>\<o>\<r>\<m>\<s> U \<r>\<e>\<m>\<a>\<i>\<n>\<s>[C] R \<s>\<u>\<b>\<j> Q \<w>\<i>\<t>\<h> P"
   unfolding Transformation_def Premise_def by simp blast
 
